compiler proof done

src/Pyrosome/Lang/Multilanguages.v
@@ -5,6 +5,13 @@ Import ListNotations.
 Open Scope string.
 Open Scope list.
 From Utils Require Import Utils.
+
+(* imports for compilers *)
+(* copied from LinearCPS.v *)
+From Pyrosome Require Import Compilers.Compilers Elab.ElabCompilers.
+Import CompilerDefs.Notations. (* for `match # from high_level_multilanguage with` *)
+(* CompilerDefs, for preserving_compiler_ext, is already imported. Prolly through something else. *)
+
 From Pyrosome Require Import Theory.Core Elab.Elab
   Tools.Matches
   Tools.EGraph.TypeInference Tools.Resolution Tools.EGraph.ComputeWf.
@@ -23,12 +30,6 @@ From Pyrosome.Lang Require Import PolySubst SimpleVSubst.
 From Pyrosome.Lang Require Import PolyCompilers. (* for parameterizing existing languages*)
 From Pyrosome.Compilers Require Import Parameterizer.
 Import Pyrosome.Tools.UnElab. 
-
-(* imports for compilers *)
-(* copied from LinearCPS.v *)
-From Pyrosome Require Import Compilers.Compilers Elab.ElabCompilers.
-Import CompilerDefs.Notations. (* for `match # from high_level_multilanguage with` *)
-(* CompilerDefs, for preserving_compiler_ext, is already imported. Prolly through something else. *)
 
 Definition boundaries_def : lang :=
   {[l/subst [exp_subst++value_subst] 
@@ -183,12 +184,9 @@ Proof. solve_parameterize_wrapper typed_bool. Qed.
 
 Definition typed_bool_ty_subst_def := Eval vm_compute in (eqn_rules
   type_subst_mode
-    (exp_param_substs ++
-     exp_ty_subst ++
-     val_param_substs ++
-     val_ty_subst ++
-     env_ty_subst ++
-     ty_subst_lang ++
+    (exp_param_substs ++ exp_ty_subst ++
+     val_param_substs ++ val_ty_subst ++
+     env_ty_subst ++ ty_subst_lang ++
      exp_parameterized ++ val_parameterized ++ ty_env_lang
     )
     (hide_lang_implicits (typed_bool_parameterized ++
@@ -203,12 +201,9 @@ Definition typed_bool_ty_subst_def := Eval vm_compute in (eqn_rules
        typed_bool_parameterized)).
 Derive typed_bool_ty_subst
   SuchThat (elab_lang_ext (typed_bool_parameterized ++
-                                exp_param_substs ++
-                                exp_ty_subst ++
-                                val_param_substs ++
-                                val_ty_subst ++
-                                env_ty_subst ++
-                                ty_subst_lang ++
+                                exp_param_substs ++ exp_ty_subst ++
+                                val_param_substs ++ val_ty_subst ++
+                                env_ty_subst ++ ty_subst_lang ++
                                 exp_parameterized ++ val_parameterized ++ ty_env_lang
                                 )
               typed_bool_ty_subst_def typed_bool_ty_subst)
@@ -220,34 +215,25 @@ Proof. auto_elab. Qed.
 
 Definition stlc_ty_subst_def := Eval vm_compute in (eqn_rules
   type_subst_mode
-    (exp_param_substs ++
-     exp_ty_subst ++
-     val_param_substs ++
-     val_ty_subst ++
-     env_ty_subst ++
-     ty_subst_lang ++
+    (exp_param_substs ++ exp_ty_subst ++
+     val_param_substs ++ val_ty_subst ++
+     env_ty_subst ++ ty_subst_lang ++
      exp_parameterized ++ val_parameterized ++ ty_env_lang
     )
     (hide_lang_implicits (stlc_parameterized ++
-                            exp_param_substs ++
-                            exp_ty_subst ++
-                            val_param_substs ++
-                            val_ty_subst ++
-                            env_ty_subst ++
-                            ty_subst_lang ++
+                            exp_param_substs ++ exp_ty_subst ++
+                            val_param_substs ++ val_ty_subst ++
+                            env_ty_subst ++ ty_subst_lang ++
                             exp_parameterized ++ val_parameterized ++ ty_env_lang
        )
        stlc_parameterized)).
 Derive stlc_ty_subst
   SuchThat (elab_lang_ext (stlc_parameterized ++
-                             exp_param_substs ++
-                             exp_ty_subst ++
-                             val_param_substs ++
-                             val_ty_subst ++
-                             env_ty_subst ++
-                             ty_subst_lang ++
+                             exp_param_substs ++ exp_ty_subst ++
+                             val_param_substs ++ val_ty_subst ++
+                             env_ty_subst ++ ty_subst_lang ++
                              exp_parameterized ++ val_parameterized ++ ty_env_lang
-                                )
+              )
               stlc_ty_subst_def stlc_ty_subst)
   As stlc_ty_subst_wf.
 Proof. auto_elab. Qed.
@@ -276,25 +262,19 @@ Definition usubst_ty_subst_def := Eval vm_compute in (eqn_rules
      exp_parameterized ++ val_parameterized ++ ty_env_lang
     )
     (hide_lang_implicits (usubst_parameterized ++
-                            exp_param_substs ++
-                            exp_ty_subst ++
-                            val_param_substs ++
-                            val_ty_subst ++
-                            env_ty_subst ++
-                            ty_subst_lang ++
+                            exp_param_substs ++ exp_ty_subst ++
+                            val_param_substs ++ val_ty_subst ++
+                            env_ty_subst ++ ty_subst_lang ++
                             exp_parameterized ++ val_parameterized ++ ty_env_lang
        )
        usubst_parameterized)).
 Derive usubst_ty_subst
   SuchThat (elab_lang_ext (usubst_parameterized ++
-                                exp_param_substs ++
-                                exp_ty_subst ++
-                                val_param_substs ++
-                                val_ty_subst ++
-                                env_ty_subst ++
-                                ty_subst_lang ++
+                                exp_param_substs ++ exp_ty_subst ++
+                                val_param_substs ++ val_ty_subst ++
+                                env_ty_subst ++ ty_subst_lang ++
                                 exp_parameterized ++ val_parameterized ++ ty_env_lang
-                                )
+              )
               usubst_ty_subst_def usubst_ty_subst)
   As usubst_ty_subst_wf.
 Proof. auto_elab. Qed.
@@ -404,12 +384,9 @@ Derive type_casing
                   usubst_parameterized ++
                   poly ++ (* needed for #"All" *)
                   (* below are the things needed for polymorphic languages *)
-                  exp_param_substs ++
-                  exp_ty_subst ++
-                  val_param_substs ++
-                  val_ty_subst ++
-                  env_ty_subst ++
-                  ty_subst_lang ++
+                  exp_param_substs ++ exp_ty_subst ++
+                  val_param_substs ++ val_ty_subst ++
+                  env_ty_subst ++ ty_subst_lang ++
                   exp_parameterized ++ val_parameterized ++ ty_env_lang
               ) 
                 type_casing_def type_casing)
@@ -641,11 +618,6 @@ Qed.
   lang_entry boolhuh_parameterized_wf.
 #[export] Hint Resolve boolhuh_parameterized_entry : wf_lang_db.
 
-Compute boolhuh_parameterized. 
-
-(*
-
-
 Definition boolhuh_ty_subst_def := Eval vm_compute in (eqn_rules
   type_subst_mode
   ( (* add all dependencies with their ty_subst versions *)
@@ -680,23 +652,6 @@ Definition boolhuh_ty_subst_def := Eval vm_compute in (eqn_rules
      exp_parameterized ++ val_parameterized ++ ty_env_lang
        )
      boolhuh_parameterized)). (* change this line to the current parameterized langauge working on *)
-
-
-(* Definition boolhuh_ty_subst_def : lang :=
-  {[l
-      [:= "D" : #"ty_env",
-           "D'" : #"ty_env",
-             "G" : #"env" "D",
-               "d" : #"ty_sub" "D'" "D",
-            "e" : #"exp" "D" "G" #"*"
-            ----------------------------------------------- ("exp_ty_subst bool?")
-            #"exp_ty_subst" "d" (#"bool?" "e") = #"bool?" (#"exp_ty_subst" "d" "e")
-             : #"exp" "D'" (#"env_ty_subst" "d" "G") (#"ty_subst" "d" #"*")
-        ]
-  ]}. *)
-
-Compute boolhuh_ty_subst_def. 
-
 Derive boolhuh_ty_subst
   SuchThat (elab_lang_ext ( (* add all dependencies with their ty_subst versions and the current parameterized lang *)
                 boolhuh_parameterized ++
@@ -718,23 +673,9 @@ Derive boolhuh_ty_subst
   As boolhuh_ty_subst_wf. (* and remember to change this *)
 Proof. 
 auto_elab. Qed. 
-#[export] Hint Resolve boolhuh_ty_subst_wf : elab_pfs. (* and remember to change this *)
-
-
-*)
-
-
-
-
-
-
-
-
-
-
-
-
-
+#[local] Definition boolhuh_ty_subst_entry :=
+  lang_entry (elab_lang_implies_wf boolhuh_ty_subst_wf).
+#[export] Hint Resolve boolhuh_ty_subst_entry : wf_lang_db.
 
 (* NOTE: utlc_bool does not need a ty_subst lang because there are no new syntactic constructs in utlc_bool *)
 Definition utlc_bool_parameterized := 
@@ -787,26 +728,27 @@ Definition simple_shared_fragment :=
     value_subst.
 
 Definition polymorphic_shared_fragment :=
-    boolhuh_parameterized ++  (* NOTE: MISSING BOOLHUH_TY_SUBST *)
+  boolhuh_ty_subst ++
+      boolhuh_parameterized ++
       utlc_bool_parameterized ++
       utlc_ty_subst ++
-    utlc_parameterized ++
-    untyped_bool_ty_subst ++
-    untyped_bool_parameterized ++
-    usubst_ty_subst ++
-    usubst_parameterized ++
-    typed_bool_ty_subst ++
-    typed_bool_parameterized ++
-    stlc_ty_subst ++
-    stlc_parameterized ++
-    (* all polymorphic langs stuff *) 
-    exp_param_substs ++
-    exp_ty_subst ++
-    val_param_substs ++
-    val_ty_subst ++
-    env_ty_subst ++
-    ty_subst_lang ++
-    exp_parameterized ++ val_parameterized ++ ty_env_lang.
+      utlc_parameterized ++
+      untyped_bool_ty_subst ++
+      untyped_bool_parameterized ++
+      usubst_ty_subst ++
+      usubst_parameterized ++
+      typed_bool_ty_subst ++
+      typed_bool_parameterized ++
+      stlc_ty_subst ++
+      stlc_parameterized ++
+      (* all polymorphic langs stuff *) 
+      exp_param_substs ++
+      exp_ty_subst ++
+      val_param_substs ++
+      val_ty_subst ++
+      env_ty_subst ++
+      ty_subst_lang ++
+      exp_parameterized ++ val_parameterized ++ ty_env_lang.
 
 Local Notation compiler := (compiler string).
 
@@ -899,9 +841,6 @@ Qed.
   lang_entry mif_parameterized_wf.
 #[export] Hint Resolve mif_parameterized_entry : wf_lang_db.
 
-
-(*
-
 Definition mif_ty_subst_def := Eval vm_compute in (eqn_rules
   type_subst_mode
   ( (* add all dependencies with their ty_subst versions *)
@@ -957,9 +896,9 @@ Derive mif_ty_subst
   As mif_ty_subst_wf. (* and remember to change this *)
 Proof. 
 auto_elab. Qed. 
-#[export] Hint Resolve mif_ty_subst_wf : elab_pfs. (* and remember to change this *)
-
-*)
+#[local] Definition mif_ty_subst_entry :=
+  lang_entry (elab_lang_implies_wf mif_ty_subst_wf).
+#[export] Hint Resolve mif_ty_subst_entry : wf_lang_db.
 
 Definition prod_parameterized := parameterize_wrapper prod. 
 
@@ -1010,15 +949,12 @@ Proof. auto_elab. Qed.
 
 
 Definition target_multilanguage :=
-  prod_ty_subst ++
-    prod_parameterized ++
-    mif_parameterized ++ (* NOTE: MISSING MIF_TY_SUBST *)
+  prod_ty_subst ++ prod_parameterized ++
+    mif_ty_subst ++ mif_parameterized ++ 
     type_casing ++
     poly ++
     polymorphic_shared_fragment.
 Hint Unfold target_multilanguage : auto_elab.
-
-Axiom todo_2 : wf_lang target_multilanguage.
 
 Fixpoint wkn_n n :=
   match n with
@@ -1031,6 +967,7 @@ Fixpoint wkn_n n :=
 Definition ovar n :=
     {{e #"val_subst" {wkn_n n} #"hd" }}.  
 
+(* this is not used *)
 Fixpoint vwkn_n n e :=
   match n with
   | 0 => e
@@ -1038,111 +975,41 @@ Fixpoint vwkn_n n e :=
     {{e #"val_subst" #"wkn" {vwkn_n n' e} }}
   end.
 
-(*
-Definition ttd_fun t1 (x : t1 -> dyn) t2 (y : t2 -> dyn) : (t1 -> t2) -> dyn :=
-  fun input =>
-    ufun z =>
-    y (input (dtt t1 z))
-.
-Definition ttd t : t -> dyn :=
-  match t with
-  | dyn => fun x => x
-  | bool => fun x =>  if x then utrue else ufalse
-  | t1 -> t2 => fun t1 (x : t1 -> dyn) t2 (y : t2 -> dyn) => fun input => (* x is NOT _this_ dtt! which is why the type is flipped *)
-    ufun z =>
-      y (input (dtt t1 z))
-  end.
-
-Definition dtt t : dyn -> t :=
-  match t with
-  | dyn => fun x => x
-  | bool => fun x =>  mif x then true else false
-  | t1 -> t2 => fun t1 (x : dyn -> t1) t2 (y : dyn -> t2) => ufun input =>
-    fun z =>
-      y (input (ttd t1 z))
-  end.
-
-Definition boundaries t : (t -> dyn) * (dyn -> t) :=
-  match t with
-  | dyn => (fun x => x, fun x => x)
-  | bool => (fun x =>  if x then utrue else ufalse, fun x =>  mif x then true else false)
-  | t1 -> t2 => fun t1 (x : (t1 -> dyn) * (dyn -> t1)) t2 (y : (t2 -> dyn) * (dyn -> t2)) =>
-                  (
-                    fun input =>
-    ufun z =>
-      (fst y) (input ((snd x) z))
-                    , (* above is ttd, below is dtt *)
-                    ufun input =>
-    fun z =>
-      (snd y) (input ((fst x) z))
-                    )
-  end. (* in the first case, the first thing is first of y bc we want to get the same direction, and in the second one its second *)
-(* then we reverse evertyihng in the other one *)
-*)
-(* so the way this is gonna work is that we're gonna have a typerec that has as its three cases the three things in the boundaries func *)
-
-(*
- Ltac t' :=
-  match goal with
-  | [|- fresh _ _ ]=> compute_fresh
-  | [|- sublist _ _ ]=> apply (use_sublistb); vm_compute; reflexivity
-  | |- In _ _ => solve [solve_in | simpl; intuition fail]
-  | |- Model.wf_term _ _ _ => cbn [Model.wf_term core_model]
-  | |- wf_term ?l ?c ?e ?t =>
-        let c' := eval vm_compute in c in
-        let e' := eval vm_compute in e in
-        let t' := eval vm_compute in t in
-            change_no_check (wf_term l c' e' t');
-    tryif first [has_evar c'| has_evar e' | has_evar t']
-    then assumption || eapply wf_term_var || eapply wf_term_by'
-    else compute_noconv_term_wf
-  | [|-wf_args _ _ _ _] => simple apply wf_args_nil
-                           || simple eapply wf_args_cons2
-                           || simple eapply wf_args_cons
-  | [|-wf_subst _ _ _] => constructor
-  | |- wf_ctx (Model:= ?m) ?c =>
-    let c' := eval vm_compute in c in
-        change_no_check (wf_ctx (Model:= m) c');
-    tryif has_evar c'
-    then assumption || constructor
-    else solve_wf_ctx
-  | |- wf_sort ?l ?c ?t =>
-        let c' := eval vm_compute in c in
-        let t' := eval vm_compute in t in
-        change_no_check (wf_sort l c' t'); eapply wf_sort_by
-  | [|- wf_lang _] => solve[Tools.Resolution.prove_by_lang_db]
-  (*Don't use vm_compute here*)
-  | [|- _ = _] => compute; reflexivity
-  end.
-*)
+(* it seems this is still needed *)
+Lemma target_multilanguage_wf : wf_lang target_multilanguage.
+Proof. prove_by_lang_db. Qed.
+#[local] Definition target_multilanguage_entry :=
+  lang_entry target_multilanguage_wf.
+#[export] Hint Resolve target_multilanguage_entry : wf_lang_db.
 
 Ltac derive_elab_term :=
-  pose proof todo_2;
+  pose proof target_multilanguage_wf;
   unshelve (repeat t); t'. (* repeat t then unshelve; then on the unshelved do t'. *)
 
-Derive bool_test
-  in (elab_term target_multilanguage
-                [("G", {{s #"env" #"ty_emp"}})]
-         {{e #"lambda" #"bool" (#"ret" #"T") }}
-         bool_test
-         {{s #"exp" #"ty_emp" "G"
-                (#"->" #"ty_emp" (#"bool" #"ty_emp") (#"bool" #"ty_emp"))
-         }}
-     ) as bool_test_wf.
-Proof.
-  pose proof todo_2.
-  repeat t.
-  1: solve_in.
-  
-  1: solve [ solve_in | simpl; intuition fail ]. 
+Ltac solve_eq_sort_disj :=
+  right; compute_eq_compilation; sort_cong; repeat by_reduction.
 
+Ltac mega_derive_elab_term :=
+  pose proof target_multilanguage_wf;
+  (* NOTE: the by_reduction below seems to me redundant given the def of solve_eq_sort_disj, but it's necessary for trec_boundaries and for both elab_term goals in the compiler *)
+  (* the elab_term goals in the compiler were goals that I had to do out of order. Wonder if that has to do with it? *)
+  (* and now that I think about it, the way I was doing the elab_term goals in trec_boundaries was doing the last one first. Then the rest went through. So it does seem like an order thing... but this solves it? *)
+  unshelve (repeat t; solve_eq_sort_disj; by_reduction); t'.
+
+(* tactic to see if progress can be made on an elab_term goal *)
+Ltac quick_goal_match :=
+  lazymatch goal with
+  | |- elab_term _ _ (con ?s _) (con ?s _) _ =>
+      idtac "can go further"
+  | |- elab_term _ _ (con ?s _) (con ?s' _) _ =>
+      fail "cannot go further"
+  | |- _  => idtac "neither case"
+  end.
 
 Definition trec_star_case_unelab :=
-  {{e
-      #"pair"
+  {{e #"pair"
       (#"ret" (#"lambda" #"*" (#"ret" #"hd")))
-      (#"ret" (#"lambda" #"*" (#"ret" #"hd")))
-  }}.
+      (#"ret" (#"lambda" #"*" (#"ret" #"hd"))) }}.
 Derive trec_star_case
   in ( elab_term target_multilanguage
          [("G", {{s #"env" #"ty_emp"}})]
@@ -1155,28 +1022,12 @@ Derive trec_star_case
              )
          }}
      ) as trec_star_case_wf.
-Proof.
-  pose proof todo_2.
-  repeat t. 
-  unshelve (repeat t).
-  Print Matches.t'. 
-  all: try apply default.
-  Print t'.
-  1: solve_in. 
-  1: solve [ solve_in | simpl; intuition fail ].
-  Print t'. 
-  18: t'. 
-  
-  all: try t'. 
-
-  derive_elab_term. Qed.
+Proof. derive_elab_term. Qed. 
 
 Definition trec_bool_case_unelab :=
-  {{e
-      #"pair"
+  {{e #"pair"
       (#"ret" (#"lambda" #"bool" (#"if" (#"ret" #"hd") (#"ret" #"uT") (#"ret" #"uF"))))
-      (#"ret" (#"lambda" #"*" (#"mif" (#"ret" #"hd") (#"ret" #"T") (#"ret" #"F"))))
-  }}. 
+      (#"ret" (#"lambda" #"*" (#"mif" (#"ret" #"hd") (#"ret" #"T") (#"ret" #"F")))) }}. 
 Derive trec_bool_case
   in ( elab_term target_multilanguage
          [("G", {{s #"env" #"ty_emp"}})]
@@ -1191,339 +1042,22 @@ Derive trec_bool_case
      ) as trec_bool_case_wf. 
 Proof. derive_elab_term. Qed.
 
-Ltac quick_goal_match :=
-  lazymatch goal with
-  | |- elab_term _ _ (con ?s _) (con ?s _) _ =>
-      idtac "can go further"
-  | |- elab_term _ _ (con ?s _) (con ?s' _) _ =>
-      fail "cannot go further"
-  | |- _  => idtac "neither case"
-  end.
-
-(*
-Definition trec_func_case'_unelab :=
-  {{e
-      #"pair"
-         (#"ret"
-            (#"lambda" (#"->" "t1" "t2")
-               (#"ret"
-                  (#"ulambda"
-                     (#"app" (#".1" (#"ret" "v2")) (#"app" (#"ret" {ovar 1}) (#"app" (#".2" (#"ret" "v3")) (#"ret" {ovar 0}))))
-                  )
-               )
-            )
-         )
-         (#"ret"
-            (#"lambda" #"*"
-               (#"ret"
-                  (#"lambda" "t1"
-                     (#"app" (#".2" (#"ret" "v2")) (#"uapp" (#"ret" {ovar 1}) (#"app" (#".1" (#"ret" "v3")) (#"ret" {ovar 0}))))
-                  )
-               )
-            )
-         )
-  }}.
-
-Definition two_var_env := {{e #"ty_ext" (#"ty_ext" #"ty_emp") }}.
-Derive trec_func_case'_sort
-  in (elab_sort target_multilanguage
-        [
-           ("G", {{s #"env" #"ty_emp"}});
-           ("t1", {{s #"ty" (#"ty_ext" #"ty_emp") "G"}});
-           ("t2", {{s #"ty" (#"ty_ext" (#"ty_ext" #"ty_emp")) "G"}});
-           ("v2", {{s #"val" {two_var_env} "G"
-                      (#"prod" {two_var_env}
-                         (#"->" {two_var_env} "t2" (#"*" {two_var_env}))
-                         (#"->" {two_var_env} (#"*" {two_var_env}) "t2")
-                      )
-           }});
-           ("v3", {{s #"val" {two_var_env} "G"
-                      (#"prod" {two_var_env}
-                         (#"->" {two_var_env} "t1" (#"*" {two_var_env}))
-                         (#"->" {two_var_env} (#"*" {two_var_env}) "t1")
-                      )
-           }})
-         ]
-        {{s #"exp" #"ty_emp" "G"
-             (#"All" 
-                (#"->" (#"prod" (#"->" {ty_ovar 0} #"*") (#"->" #"*" {ty_ovar 0}))
-                   (#"All"
-                      (#"->" (#"prod" (#"->" {ty_ovar 0} #"*") (#"->" #"*" {ty_ovar 0}))
-                             (#"prod" (#"->" (#"->" {ty_ovar 1} {ty_ovar 0}) #"*") (#"->" #"*" (#"->" {ty_ovar 1} {ty_ovar 0})))
-                      )
-                   )
-                )
-             )
-        }}
-        trec_func_case'_sort
- 
-     )
-    as trec_func_case_sort_wf.
-Proof.
-  pose proof todo_2.
-  repeat t.
-  all: t'.
-  Abort. 
-
-
-Derive trec_func_case'
-  in ( elab_term target_multilanguage
-         [
-           ("G", {{s #"env" #"ty_emp"}});
-           ("t1", {{s #"ty" (#"ty_ext" #"ty_emp") "G"}});
-           ("t2", {{s #"ty" (#"ty_ext" (#"ty_ext" #"ty_emp")) "G"}});
-           ("v2", {{s #"val" {two_var_env} "G"
-                      (#"prod" {two_var_env}
-                         (#"->" {two_var_env} "t2" (#"*" {two_var_env}))
-                         (#"->" {two_var_env} (#"*" {two_var_env}) "t2")
-                      )
-           }});
-           ("v3", {{s #"val" {two_var_env} "G"
-                      (#"prod" {two_var_env}
-                         (#"->" {two_var_env} "t1" (#"*" {two_var_env}))
-                         (#"->" {two_var_env} (#"*" {two_var_env}) "t1")
-                      )
-           }})
-         ]
-         trec_func_case'_unelab
-         trec_func_case'
-         {{s #"exp" #"ty_emp" "G"
-                             (#"prod" (#"->" (#"->" "t1" "t2") #"*") (#"->" #"*" (#"->" "t1" "t2")))
-         }}
-     ) as trec_func_case_wf.
-Proof.
-  pose proof todo_2.
-  repeat t.
-  Abort. 
-*)
-
-
-
-
 Derive trec_func_case_sort
   in (elab_sort target_multilanguage
         [("G", {{s #"env" #"ty_emp"}})]
         {{s #"exp" #"ty_emp" "G"
-             (#"All" 
-                (#"->" (#"prod" (#"->" {ty_ovar 0} #"*") (#"->" #"*" {ty_ovar 0}))
-                   (#"All"
-                      (#"->" (#"prod" (#"->" {ty_ovar 0} #"*") (#"->" #"*" {ty_ovar 0}))
-                             (#"prod" (#"->" (#"->" {ty_ovar 1} {ty_ovar 0}) #"*") (#"->" #"*" (#"->" {ty_ovar 1} {ty_ovar 0})))
-                      )
-                   )
-                )
-             )
-        }}
+            (#"All" 
+               (#"->" (#"prod" (#"->" {ty_ovar 0} #"*") (#"->" #"*" {ty_ovar 0}))
+                  (#"All"
+                     (#"->" (#"prod" (#"->" {ty_ovar 0} #"*") (#"->" #"*" {ty_ovar 0}))
+                        (#"prod" (#"->" (#"->" {ty_ovar 1} {ty_ovar 0}) #"*") (#"->" #"*" (#"->" {ty_ovar 1} {ty_ovar 0}))))))) }}
         trec_func_case_sort
      )
     as trec_func_case_sort_wf.
 Proof. derive_elab_term. Qed.
 
-Print trec_func_case_sort.
-
 Definition trec_func_case_unelab :=
-  {{e
-      #"ret"
-      (#"Lam"
-         (#"ret"
-            (#"lambda" (#"prod" (#"->" {ty_ovar 0} #"*") (#"->" #"*" {ty_ovar 0}))
-               (#"ret"
-                  (#"Lam"
-                     (#"ret"
-                        (#"lambda" (#"prod" (#"->" {ty_ovar 0} #"*") (#"->" #"*" {ty_ovar 0}))
-
-                           (#"pair"
-         (#"ret"
-            (#"lambda" (#"->" {ty_ovar 1} {ty_ovar 0})
-               (#"ret"
-                  (#"ulambda"
-                     (#"app" (#".1" (#"ret" {ovar 2})) (#"app" (#"ret" {ovar 1}) (#"app" (#".2" (#"ret" {ovar 3})) (#"ret" {ovar 0}))))
-                  )
-               )
-            )
-         )
-         (#"ret"
-            (#"lambda" #"*"
-               (#"ret"
-                  (#"lambda" {ty_ovar 1}
-                     (#"app" (#".2" (#"ret" {ovar 2})) (#"uapp" (#"ret" {ovar 1}) (#"app" (#".1" (#"ret" {ovar 3})) (#"ret" {ovar 0}))))
-                  )
-               )
-            )
-         )
-      )
-                        )
-                     )
-                  )
-               )
-            )
-         )
-      )
-  }}.
-
-
-
-
-
-
-
-Definition evar := {{e #"ty_emp" }}.
-Definition evar2 := {{e "G" }}. 
-Definition lhs := 
-{{s #"exp" (#"ty_ext" (#"ty_ext" {evar})) (#"ext" (#"ty_ext" (#"ty_ext" {evar})) {
-                                                    evar2} (#"prod" (#"ty_ext" (#"ty_ext" {evar})) (
-                                                                  #"->" (
-                                                                        #"ty_ext" (#"ty_ext" {evar})) (
-                                                                        #"ty_subst" 
-                                                                        (
-                                                                        #"ty_ext" (#"ty_ext" {evar})) (
-                                                                        #"ty_ext" 
-                                                                        {evar}) (
-                                                                        #"ty_wkn" 
-                                                                        (#"ty_ext" {evar})) (
-                                                                        #"ty_hd" 
-                                                                        {evar})) (
-                                                                        #"*" 
-                                                                        (
-                                                                        #"ty_ext" (#"ty_ext" {evar})))) (
-                                                                  #"->" (
-                                                                        #"ty_ext" (#"ty_ext" {evar})) (
-                                                                        #"*" 
-                                                                        (
-                                                                        #"ty_ext" (#"ty_ext" {evar}))) (
-                                                                        #"ty_subst" 
-                                                                        (
-                                                                        #"ty_ext" (#"ty_ext" {evar})) (
-                                                                        #"ty_ext" 
-                                                                        {evar}) (
-                                                                        #"ty_wkn" 
-                                                                        (#"ty_ext" {evar})) (
-                                                                        #"ty_hd" 
-                                                                        {evar}))))) (
-             #"->" (#"ty_ext" (#"ty_ext" {evar})) (#"prod" (#"ty_ext" (#"ty_ext" {evar})) (
-                                                           #"->" (#"ty_ext" (#"ty_ext" {evar})) (
-                                                                 #"ty_hd" 
-                                                                 (#"ty_ext" {evar})) (
-                                                                 #"*" (#"ty_ext" (#"ty_ext" {evar})))) (
-                                                           #"->" (#"ty_ext" (#"ty_ext" {evar})) (
-                                                                 #"*" (#"ty_ext" (#"ty_ext" {evar}))) (
-                                                                 #"ty_hd" 
-                                                                 (#"ty_ext" {evar})))) (
-                   #"prod" (#"ty_ext" (#"ty_ext" {evar})) (#"->" (#"ty_ext" (#"ty_ext" {evar})) (
-                                                                 #"->" (#"ty_ext" (#"ty_ext" {evar})) (
-                                                                       #"ty_subst" 
-                                                                       (#"ty_ext" (#"ty_ext" {evar})) (
-                                                                       #"ty_ext" 
-                                                                       {evar}) (
-                                                                       #"ty_wkn" 
-                                                                       (#"ty_ext" {evar})) (
-                                                                       #"ty_hd" 
-                                                                       {evar})) (
-                                                                       #"ty_hd" 
-                                                                       (#"ty_ext" {evar}))) (
-                                                                 #"*" (#"ty_ext" (#"ty_ext" {evar})))) (
-                           #"->" (#"ty_ext" (#"ty_ext" {evar})) (#"*" (#"ty_ext" (#"ty_ext" {evar}))) (
-                                 #"->" (#"ty_ext" (#"ty_ext" {evar})) (#"ty_subst" 
-                                                                       (#"ty_ext" (#"ty_ext" {evar})) (
-                                                                       #"ty_ext" 
-                                                                       {evar}) (
-                                                                       #"ty_wkn" 
-                                                                       (#"ty_ext" {evar})) (
-                                                                       #"ty_hd" 
-                                                                       {evar})) (
-                                     #"ty_hd" (#"ty_ext" {evar}))))))}}.
-
-Definition rhs := {{s #"exp" (#"ty_ext" (#"ty_ext" #"ty_emp")) (#"env_ty_subst" (#"ty_ext" (#"ty_ext" #"ty_emp")) (
-                                                                #"ty_ext" 
-                                                                #"ty_emp") (
-                                                                #"ty_wkn" 
-                                                                (#"ty_ext" #"ty_emp")) (
-                                                                #"ext" (#"ty_ext" #"ty_emp") (
-                                                                       #"env_ty_subst" 
-                                                                       (#"ty_ext" #"ty_emp") #"ty_emp" (
-                                                                       #"ty_wkn" 
-                                                                       #"ty_emp") "G") (
-                                                                       #"prod" 
-                                                                       (#"ty_ext" #"ty_emp") (
-                                                                       #"->" 
-                                                                       (#"ty_ext" #"ty_emp") (
-                                                                       #"ty_hd" 
-                                                                       #"ty_emp") (
-                                                                       #"*" 
-                                                                       (#"ty_ext" #"ty_emp"))) (
-                                                                       #"->" 
-                                                                       (#"ty_ext" #"ty_emp") (
-                                                                       #"*" 
-                                                                       (#"ty_ext" #"ty_emp")) (
-                                                                       #"ty_hd" 
-                                                                       #"ty_emp"))))) (
-             #"->" (#"ty_ext" (#"ty_ext" #"ty_emp")) (#"prod" (#"ty_ext" (#"ty_ext" #"ty_emp")) (
-                                                              #"->" (#"ty_ext" (#"ty_ext" #"ty_emp")) (
-                                                                    #"ty_hd" 
-                                                                    (#"ty_ext" #"ty_emp")) (
-                                                                    #"*" 
-                                                                    (#"ty_ext" (#"ty_ext" #"ty_emp")))) (
-                                                              #"->" (#"ty_ext" (#"ty_ext" #"ty_emp")) (
-                                                                    #"*" 
-                                                                    (#"ty_ext" (#"ty_ext" #"ty_emp"))) (
-                                                                    #"ty_hd" 
-                                                                    (#"ty_ext" #"ty_emp")))) (
-                   #"prod" (#"ty_ext" (#"ty_ext" #"ty_emp")) (#"->" (#"ty_ext" (#"ty_ext" #"ty_emp")) (
-                                                                    #"->" 
-                                                                    (#"ty_ext" (#"ty_ext" #"ty_emp")) (
-                                                                    #"ty_subst" 
-                                                                    (#"ty_ext" (#"ty_ext" #"ty_emp")) (
-                                                                    #"ty_ext" 
-                                                                    #"ty_emp") (
-                                                                    #"ty_wkn" 
-                                                                    (#"ty_ext" #"ty_emp")) (
-                                                                    #"ty_hd" 
-                                                                    #"ty_emp")) (
-                                                                    #"ty_hd" 
-                                                                    (#"ty_ext" #"ty_emp"))) (
-                                                                    #"*" 
-                                                                    (#"ty_ext" (#"ty_ext" #"ty_emp")))) (
-                           #"->" (#"ty_ext" (#"ty_ext" #"ty_emp")) (#"*" 
-                                                                    (#"ty_ext" (#"ty_ext" #"ty_emp"))) (
-                                 #"->" (#"ty_ext" (#"ty_ext" #"ty_emp")) (
-                                       #"ty_subst" (#"ty_ext" (#"ty_ext" #"ty_emp")) (
-                                                   #"ty_ext" #"ty_emp") (
-                                                   #"ty_wkn" (#"ty_ext" #"ty_emp")) (
-                                                   #"ty_hd" #"ty_emp")) (
-                                     #"ty_hd" (#"ty_ext" #"ty_emp"))))))}}.
-
-Check eq_sort.
-
-Ltac hide_implicits_custom :=
-  lazymatch goal with
-  | |- Model.eq_sort ?l ?c ?s1 ?s2 =>
-        let c' := eval compute in (hide_ctx_implicits l c) in
-        let s1' := eval compute in (hide_sort_implicits l s1) in
-        let s2' := eval compute in (hide_sort_implicits l s2) in
-        change (Model.eq_sort l (!! as_ctx c') (!! s1') (!! s2'))
-  end.
-
-
-Theorem problem_case : eq_sort
-                         target_multilanguage
-                         {{c "G" : #"env" #"ty_emp" }}
-                         lhs
-                         rhs.
-Proof.
-  pose proof todo_2. 
-  compute.
-  
-  sort_cong.
-  1: by_reduction.
-  2: by_reduction.
-  (* there's one goal left, and it's a env_ty_subst on one side and an ext on the other side *)
-  Abort. 
-  
-
-
-
-
-
+  {{e #"ret" (#"Lam" (#"ret" (#"lambda" (#"prod" (#"->" {ty_ovar 0} #"*") (#"->" #"*" {ty_ovar 0})) (#"ret" (#"Lam" (#"ret" (#"lambda" (#"prod" (#"->" {ty_ovar 0} #"*") (#"->" #"*" {ty_ovar 0})) (#"pair" (#"ret" (#"lambda" (#"->" {ty_ovar 1} {ty_ovar 0}) (#"ret" (#"ulambda" (#"app" (#".1" (#"ret" {ovar 2})) (#"app" (#"ret" {ovar 1}) (#"app" (#".2" (#"ret" {ovar 3})) (#"ret" {ovar 0})))))))) (#"ret" (#"lambda" #"*" (#"ret" (#"lambda" {ty_ovar 1} (#"app" (#".2" (#"ret" {ovar 2})) (#"uapp" (#"ret" {ovar 1}) (#"app" (#".1" (#"ret" {ovar 3})) (#"ret" {ovar 0})))) ) ))))))))))) }}.
 Derive trec_func_case
   in ( elab_term target_multilanguage
          [("G", {{s #"env" #"ty_emp"}})]
@@ -1531,114 +1065,33 @@ Derive trec_func_case
          trec_func_case
          trec_func_case_sort
      ) as trec_func_case_wf.
-Proof.
-  pose proof todo_2.
-  repeat t.
-  right.
-  compute_eq_compilation.
-  sort_cong.
-  1: term_refl.
-  1: compute_eq_compilation.
-  1: reduce.
-  1: term_cong.
-  1: term_refl.
-  1: reduce.
-  1: term_refl.
-  1: by_reduction.
-  1: compute_eq_compilation.
-  term_cong.
-  1: term_refl.
-  1: compute_eq_compilation.
-  1: term_cong.
-  1: term_refl.
-  1: term_refl.
-  1: term_refl.
-  compute_eq_compilation.
-  term_refl.
-  Unshelve.
-  all: t'.
-Qed.
-
-
+Proof. mega_derive_elab_term. Qed.
 
 Definition trec_boundaries_unelab :=
-  {{e
-      #"typerec" "A" (#"prod" (#"->" {ty_ovar 0} #"*") (#"->" #"*" {ty_ovar 0}))
+  {{e #"typerec" "A" (#"prod" (#"->" {ty_ovar 0} #"*") (#"->" #"*" {ty_ovar 0}))
       {trec_star_case_unelab}
       {trec_bool_case_unelab}
-      {trec_func_case_unelab}
-  }}.
-
+      {trec_func_case_unelab} }}.
 Derive trec_boundaries
          in ( elab_term target_multilanguage
-                [("e", {{s #"exp" #"ty_emp" "G" "A"}}); ("A", {{s #"ty" #"ty_emp"}});
-
-                 ("G", {{s #"env" #"ty_emp"}})]
+                [("A", {{s #"ty" #"ty_emp"}}); ("G", {{s #"env" #"ty_emp"}})]
                 trec_boundaries_unelab
                 trec_boundaries
                 {{s #"exp" #"ty_emp" "G"
                     (#"prod" #"ty_emp"
                        (#"->" #"ty_emp" "A" (#"*" #"ty_emp"))
-                       (#"->" #"ty_emp" (#"*" #"ty_emp") "A")
-                    )
-                }}
+                       (#"->" #"ty_emp" (#"*" #"ty_emp") "A")) }}
             ) as trec_boundaries_wf.
-Proof.
-Abort.
-(* 
-  derive_elab_term. 
-  t.
-  2: t. 2: t. 2: t.
-  3: t. 3: t. 3: t.
-  4: t. 4: t. 4: t.
-  5: t. 5: t. 5: t.
-  6: t. 6: t. 6: t.
-  7: t. 7: t. 7: t.
-  8: t. 8: t. 8: t.
-  9: t. 9: t. 9: t.
-  10: t. 10: t. 10: t.
-  11: t. 11: t. 11: t.
-  12: t. 12: t. 12: t.
-  13: t. 13: t. 13: t.
-  14: t. 14: t. 14: t.
-  15: t. 15: t. 15: t.
-  16: t. 16: t. 16: t.
-  17: t. 17: t. 17: t.
-  18: t.
+Proof. mega_derive_elab_term. Qed.
 
-  Compute target_multilanguage. 
-  18: t. 18: t.
-  19: t. 19: t. 19: t.
-  20: t. 20: t. 20: t.
-  21: t. 21: t. 21: t.
-  22: t. 22: t. 22: t.
-  23: t. 23: t. 23: t.
-  24: t. 24: t. 24: t.
-  25: t. 25: t. 25: t.
-  26: t. 26: t. 26: t.
-  27: t. 27: t. 27: t.
-  28: t. 28: t. 28: t.
-  29: t. 29: t. 29: t.
-
-  repeat Matches.t.
-  Qed. 
-  Matches.t. 1: Matches.t. 2: shelve. t. 1: repeat t. 2: t. 2: repeat t. 3: repeat t.
-  all: cycle 1. 1: t.
-  Compute prod_parameterized. 
-  1: solve_in.
-  1: t. 1: repeat t. 2: repeat t. 
-  all: try (left; reflexivity).
- *)  
-
-
-(*
 (* simple to poly compiler *)
 Definition multilang_compiler_def : compiler :=
     match # from (boundaries ++ uif) with
     | {{e #"uif" "G" "c" "thn" "els"}} => {{e @"mif" @("D" := #"ty_emp") "c" "thn" "els" }}
-    | {{e #"dtt" "G" "A" "e"}} => {{e #"app" (#".2" {trec_boundaries {{e "A"}}}) "e" }}
-    | {{e #"ttd" "G" "A" "e"}} => {{e #"app" (#".1" {trec_boundaries {{e "A"}}}) "e" }}
-    (* order of implicit vars is order of context vars *)
+    | {{e #"dtt" "G" "A" "e"}} => {{e @"app" @("D" := #"ty_emp")
+                                      (#".2" {trec_boundaries_unelab}) "e" }}
+    | {{e #"ttd" "G" "A" "e"}} => {{e @"app" @("D" := #"ty_emp")
+                                      (#".1" {trec_boundaries_unelab}) "e" }}
     end.
 
 Derive multilang_compiler 
@@ -1651,67 +1104,25 @@ Derive multilang_compiler
                     ) 
         As multilang_compiler_preserving. 
 Proof.
-  assert (wf_lang target_multilanguage) by apply todo_2.
   setup_elab_compiler.
-  { repeat Matches.t.  }
+  { derive_elab_term. }
   { by_reduction. }
   { by_reduction. }
   { by_reduction. }
   { by_reduction. }
   { by_reduction. }
-  { Compute (compile_ctx (nth_tail 2 multilang_compiler ++ shared_fragment_compiler)
-               {{c "G" : #"env", "A" : #"ty", "e" : #"exp" "G" "A"}}).
-    Compute (compile_sort (nth_tail 2 multilang_compiler ++ shared_fragment_compiler)
-       {{s #"exp" "G" #"*"}}).
+  { mega_derive_elab_term. }
+  2: mega_derive_elab_term. 
+  all: Automation.by_reduction.
+  Unshelve. all: t'.
+Qed. 
 
 
 
-      repeat Matches.t. }
-  { by_reduction. }
-  { by_reduction. }
-  { by_reduction. }
-  { by_reduction. }
-  { by_reduction. }
-  { by_reduction. }
-  { by_reduction. }
-  { by_reduction. }
-  3: { compute_eq_compilation. by_reduction.  }.
-   repeat
-    ([>repeat Matches.t; cleanup_elab_after
-        try (try decompose_sort_eq; (solve [ by_reduction ]))
-     | .. ])
-
-
-  Print auto_elab_compiler. 
-  auto_elab_compiler.
-  Check eq_term.
-  Print boundaries. 
-  setup_elab_compiler.
-   repeat
-    ([>repeat Matches.t; cleanup_elab_after
-        try (try decompose_sort_eq; (solve [ by_reduction ]))
-     | .. ])
 
 
 (* in case needed, defined in Tools.Matches, Elab.ElabCompilers *)
 (* semantic properties are in SemanticsPreservingDefs.v *)
-
-(* Locate elab_preserving_compiler. 
-Locate auto_elab_compiler.  *)
-
-Derive multilang_compiler 
-        SuchThat (elab_preserving_compiler 
-                    shared_fragment_compiler
-                    target_multilanguage
-                    multilang_compiler_def
-                    multilang_compiler
-                    (boundaries ++ uif)
-                    ) 
-        As multilang_compiler_preserving. 
-Proof. 
-Abort. 
-
-
 
 
 
@@ -1734,6 +1145,10 @@ Qed.
 Hint Resolve polymorphic_shared_fragment_identity_compiler_preserving : auto_elab.
 *)
 
+
+
+
+(* 
 Definition boundaries_parameterized_def : lang :=
   {[l
     [:| "D" : #"ty_env",
@@ -1877,9 +1292,7 @@ Derive boundaries_parameterized  (* need polymorphic versions of all these *)
         As boundaries_parameterized_wf.
 Proof. Abort. 
 (* #[export] Hint Resolve boundaries_parameterized_wf : elab_pfs. *)
-
-
-
+*)
 
 
 
@@ -1905,6 +1318,8 @@ Proof. unfold low_level_multilanguage. unfold high_level_multilanguage.
         end. 
 Admitted. 
 #[export] Hint Resolve h2l_preserving : elab_pfs. *)
+
+
 
 (* accompanying story: boundaries aren't really necessary to do multilanguages
 because they can be expressed in terms of more primitive features, but we can do mif *)
@@ -1971,5 +1386,3 @@ Definition ttd_v {G : term} (x : term) (Ty : term) : Ty :=
                      end
   | {{e #"->" {A} {B} }} => {{e #"ulambda" {ttd_e {{e #"app" (#"val_subst" #"wkn" #"ret" {x}) {dtt_e {{e #"hd"}} A} }} B} }}
   end.  *)
-
- *)
